aa

Ex2.dfy
@@ -1,27 +1,66 @@
-
 include "Ex1.dfy"
 
-class PriQueue {
-  var fst : PVNode?; 
+module Ex2 {
+  import Ex1=Ex1
 
-  ghost var pvs: multiset<(int,int)>;
-  ghost var footprint : set<PVNode>;
+  class PriQueue {
+    var fst : Ex1.PVNode?; 
 
-  function ValidQ() : bool
-    reads this, fst, if fst == null then {} else fst.footprint
-  {
-  }
-  
-  method enqueue (pri: int, v: int)
-    requires pri >= 0 && ValidQ()
-    ensures ValidQ()
-    ensures pvs == old(pvs) + multiset{(pri,v)}
-    modifies this, this.footprint
-  {
-  }
+    ghost var pvs: multiset<(int,int)>;
+    ghost var footprint : set<Ex1.PVNode>;
 
-  method dequeue () returns (r : (int, int)) 
-  {
+    function ValidQ() : bool
+      reads this, fst, if fst == null then {} else fst.footprint
+    {
+      (fst == null ==> (|pvs| == 0 && |footprint| == 0)) &&
+      (fst != null ==> (fst.Valid() && fst.footprint == footprint && multiset(fst.list) == pvs))
+    }
+    
+    method enqueue (pri: int, v: int)
+      requires pri >= 0 && ValidQ() && pri >= 0
+      ensures ValidQ()
+      ensures pvs == old(pvs) + multiset{(pri,v)}
+      modifies this, this.footprint
+    {
+      if (fst == null) {
+        fst := new Ex1.PVNode(pri, v);
+        footprint := {fst};
+        pvs := multiset{(pri, v)};
+        return;
+      } else {
+        var aux := fst.insertPVPair(pri, v);
+        footprint := aux.footprint;
+        pvs := pvs + multiset{(pri, v)};
+        fst := aux;
+        return;
+      }
+    }
+
+    method dequeue () returns (r : (int, int))
+      requires ValidQ() && fst != null
+      ensures ValidQ()
+      ensures (forall k :: k in pvs ==> k.0 <= r.0)
+      ensures old(footprint) == footprint + {old(fst)}
+      ensures old(fst) != null && old(fst).next == null ==> fst == null;
+      modifies this, footprint
+    {
+      var aux := fst.next;
+      r := (fst.pri, fst.data);
+      if (aux == null) {
+        fst := null;
+        footprint := {};
+        pvs := multiset{};
+        return;
+      } else {
+        ghost var cur := fst; 
+        assert aux.list == fst.list[1..];
+        fst := aux;
+        footprint := aux.footprint;
+        pvs := multiset(aux.list);
+        assert old(footprint) == footprint + {cur};
+        return;
+      }
+    }
+    
   }
-  
 }
