Ex4.als
@@ -6,7 +6,7 @@ sig Node {
 
 sig Queue {
 	fst: lone First,
-	last: lone Last		
+	last: lone Last	
 }
 
 sig First in Node {}
@@ -17,6 +17,7 @@ fact allNodesBelongToSomeQueue {
 	all n:Node | some q:Queue | n in q.fst.*next
 }
 
+// All nodes belong to a Queue
 fact allNodesBelongToOnlyOneQueue {
 	all n:Node, q1:Queue, q2:Queue| q1 != q2 and n in q1.fst.*next implies n !in q2.fst.*next
 }
@@ -26,17 +27,29 @@ fact lastBelongsToQueue{
 	all q:Queue | one q.fst implies q.last in q.fst.*next and one q.last
 }
 
+// All nodes' priority is smaller than the next one's
 fact NodePriority {
-	all n:Node| one n.next implies n.pri < n.next.pri
-}
-fact AllPrioritiesAreBiggerThanZero {all n:Node | n.pri > 0}
-
-
-fact p {
-	all n : Node | n not in n.^next
-	no next.First 
-	no Last.next	
+	all n:Node| one n.next implies n.pri > n.next.pri
 }
 
+// All priorities are bigger than 0
+fact AllPrioritiesAreBiggerThanZero {
+	all n:Node | n.pri >= 0
+}
+
+// No list repeats nodes (A->B->A)
+fact NoRepeatLists {
+	all n : Node | n not in n.^next	
+}
+
+// There can be no node whose next is a first node
+fact FirstNodesAreNotNext {
+	no next.First
+}
+
+// Nodes that are last in a queue have no next node
+fact NoNextInLastNode {
+	no Last.next
+}
 
 run {} for exactly 10 Node, exactly 2 Queue
